EquivModel.lean
@@ -1,0 +1,11 @@
+import UniqueList
+
+inductive equivalence_of {n : Nat} (unionList : List (Fin n × Fin n)) : Fin n → Fin n → Prop where
+| refl : (k : Fin n) → equivalence_of unionList k k
+| symm : {i j : Fin n} → equivalence_of unionList i j → equivalence_of unionList j i
+| trans : {i j k : Fin n} → equivalence_of unionList i j → equivalence_of unionList j k → equivalence_of unionList i k
+| exact : {i j : Fin n} → unionList.prop_contains ⟨i,j⟩ → equivalence_of unionList i j
+
+structure EquivModel {n : Nat} (unionList : List (Fin n × Fin n)) where
+  (query : (i j : Fin n) → Decidable (equivalence_of unionList i j))
+
